dunno?

labclasses/lab4/lab4.dfy
@@ -5,6 +5,47 @@
  * array, and the position at which the new element was inserted.
  */
 
-method sortedInsertion(a:array<int>, na:int, e:int) returns (z:array<int>,
-nz:int, pos:int)
-{}
+// method sortedInsertion(a:array<int>, na:int, e:int) returns (z:array<int>,nz:int, pos:int)
+//     requires 0 < na <= a.Length
+//     requires sorted(a, na)
+//     requires e >= 0
+//     ensures 0 < nz <= z.Length
+//     ensures sorted(z, nz)
+//     ensures pos >= 0
+// {
+ 
+// }
+
+function sortedRange(a:array<char>, l:int, h:int):bool
+    requires 0 <= l <= h <= a.Length
+    reads a
+{ forall i, j:: (l <= i < j < h) ==> a[i] <= a[j] }
+
+function sorted(a:array<char>, n:int):bool
+    requires 0 <= n <= a.Length
+    reads a
+{ forall i, j:: (0 <= i < j < n) ==> a[i] <= a[j] }
+
+
+method orderedInsert(a:array<char>, v:char, n:int)
+    requires 0 <= n < a.Length
+    requires sorted(a, n)
+    ensures sorted(a, n+1)
+    modifies a 
+{
+    if(n > 0)
+    {
+        a[n] := a[n-1];
+    }
+    var i := n;
+    while(i > 0 && v < a[i-1])
+        decreases i
+        invariant 0 <= i <= n+1
+        invariant sorted(a, n+1)
+        invariant forall k:: i < k < n+1 ==> v <= a[k]
+    {
+        a[i] := a[i-1];
+        i := i - 1;
+    }
+    a[i] := v;
+}
